Added support for conjunctions & disjunctions of primitives.

checker/coq/model.v
@@ -20,26 +20,32 @@ Inductive cst :=
   | Elem : element.ElemConstraint.(T) -> cst  
   | Cumul : cumulative.CumulConstraint.(T) -> cst  
   | Clause : clause_domain.ClauseCst.(T) -> cst
-  | Arith : arith.ArithConstraint.(T) -> cst.
+  | Arith : arith.ArithConstraint.(T) -> cst
+  | Conj : cst -> cst -> cst
+  | Disj : cst -> cst -> cst.
 
 Definition make_linear xs k := Lin (xs, k).
 Definition make_element x y ks := Elem (element.Element x y ks).
 Definition make_cumul (c : cumulative.cumul) := Cumul c.                                  
 Definition make_clause (cl : lit.clause) := Clause cl.
+Definition make_conj x y := Conj x y.
+Definition make_disj x y := Disj x y.
 
 Definition cst_id := Z.
 Definition csts := list (cst_id * cst).
 
-Definition eval_cst c (theta : valuation) := match c with
+Fixpoint eval_cst c (theta : valuation) := match c with
   | Tauto => True
   | Lin x => linear.LinearCon.(eval) x theta
   | Elem x => element.ElemConstraint.(eval) x theta
   | Cumul x => cumulative.CumulConstraint.(eval) x theta
   | Clause x => clause_domain.ClauseCst.(eval) x theta
   | Arith x => arith.ArithConstraint.(eval) x theta
+  | Conj x y => (eval_cst x theta) /\ (eval_cst y theta)
+  | Disj x y => (eval_cst x theta) \/ (eval_cst y theta)
   end.
 
-Definition check_cst_unsat c (ds : domset) := match c with
+Fixpoint check_cst_unsat c (ds : domset) := match c with
   | Tauto =>
     match ds with
       | None => true
@@ -50,14 +56,18 @@ Definition check_cst_unsat c (ds : domset) := match c with
   | Cumul x => check_unsat cumulative.CumulConstraint cumulative.CumulCheck x ds
   | Clause x => check_unsat clause_domain.ClauseCst clause_domain.ClauseCheckUnsat x ds
   | Arith x => check_unsat arith.ArithConstraint arith.ArithCheck x ds
+  | Conj x y => orb (check_cst_unsat x ds) (check_cst_unsat y ds)
+  | Disj x y => andb (check_cst_unsat x ds) (check_cst_unsat y ds)
   end.
 
 Lemma check_cst_unsat_valid : forall c ds,
   check_cst_unsat c ds = true -> forall theta, eval_domset ds theta -> eval_cst c theta -> False.                                
 Proof.
-  unfold check_cst_unsat, eval_cst; intros; destruct c;
-    try (destruct ds; tsimpl);
-    apply check_unsat_valid in H; unfold cst_is_unsat in H; specialize (H theta); tauto.
+  unfold check_cst_unsat, eval_cst; intros; induction c;
+  try (destruct ds; tsimpl);
+  try (apply check_unsat_valid in H; unfold cst_is_unsat in H; specialize (H theta); tauto).
+  (* Remaining case is conj *)
+  apply Bool.orb_true_iff in H ; destruct H as [H | H]; [apply IHc1 | apply IHc2]; intuition.
 Qed.
 
 Fixpoint eval_csts (cs : csts) (theta : valuation) := 
@@ -66,18 +76,22 @@ Fixpoint eval_csts (cs : csts) (theta : valuation) :=
   | cons c cs' => (eval_cst (snd c) theta) /\ (eval_csts cs' theta)
   end.
 
-Definition check_cst_sol c (sol : valuation) := match c with
+Fixpoint check_cst_sol c (sol : valuation) := match c with
   | Tauto => true
   | Lin x => check_sol linear.LinearCon linear.LinearSolCheck x sol
   | Elem x => check_sol element.ElemConstraint element.ElementSolCheck x sol
   | Cumul x => check_sol cumulative.CumulConstraint cumulative.CumulSolCheck x sol
   | Clause x => check_sol clause_domain.ClauseCst clause_domain.ClauseSolCheck x sol
   | Arith x => check_sol arith.ArithConstraint arith.ArithSolCheck x sol
+  | Conj x y => andb (check_cst_sol x sol) (check_cst_sol y sol)
+  | Disj x y => orb (check_cst_sol x sol) (check_cst_sol y sol)
   end.
 
 Lemma check_cst_sol_valid : forall c sol, check_cst_sol c sol = true -> eval_cst c sol.
 Proof.
-  intros c sol; unfold check_cst_sol, eval_cst; destruct c; try (trivial || apply check_sol_valid). 
+  intros c sol; unfold check_cst_sol, eval_cst; induction c; try (trivial || apply check_sol_valid). 
+  + rewrite Bool.andb_true_iff; intuition.
+  + rewrite Bool.orb_true_iff; intuition.
 Qed.
 
 Fixpoint check_csts_sol (cs : csts) sol := match cs with
